Started verifying Scheduler.yield, and am now realizing that the spec underconstrains the return pointer

platform/Scheduler.v
@@ -58,8 +58,16 @@ Module Type SCHED.
   Axiom susps_add_bwd : forall sc b pc sp, pc = pc -> mergeSusp -> susp sc pc sp * susps b sc ===> susps (b %+ (pc, sp)) sc.
   Axiom susps_del_fwd : forall sc b pc sp, (pc, sp) %in b -> susps b sc ===> susp sc pc sp * susps (b %- (pc, sp)) sc.
 
-  Axiom sched_fwd : forall sc, sched sc ===> Ex b, Ex p, sc =*> p * (sc ^+ $4) =?> 2 * queue b p * susps b sc * any.
-  Axiom sched_bwd : forall sc, (Ex b, Ex p, sc =*> p * (sc ^+ $4) =?> 2 * queue b p * susps b sc * any) ===> sched sc.
+  (* Below, the extra [locals] is a temporary stack for the scheduler to use during sensitive
+   * stack manipulations when the threads' own stacks may not be safe to touch. *)
+
+  Axiom sched_fwd : forall sc, sched sc ===> Ex b, Ex p, Ex sp, Ex vs, (sc ==*> p, sp) * (sc ^+ $8) =?> 2
+    * locals ("rp" :: "sc" :: "q" :: "curPc" :: "curSp" :: "newPc" :: "newSp" :: nil) vs 14 sp
+    * queue b p * susps b sc * any.
+
+  Axiom sched_bwd : forall sc, (Ex b, Ex p, Ex sp, Ex vs, (sc ==*> p, sp) * (sc ^+ $8) =?> 2
+    * locals ("rp" :: "sc" :: "q" :: "curPc" :: "curSp" :: "newPc" :: "newSp" :: nil) vs 14 sp
+    * queue b p * susps b sc * any) ===> sched sc.
 End SCHED.
 
 Module Sched : SCHED.
@@ -83,17 +91,23 @@ Module Sched : SCHED.
   Qed.
 
   Definition sched (sc : W) : HProp :=
-    Ex b, Ex p, sc =*> p * (sc ^+ $4) =?> 2 * queue b p * susps b sc * any.
+    Ex b, Ex p, Ex sp, Ex vs, (sc ==*> p, sp) * (sc ^+ $8) =?> 2
+      * locals ("rp" :: "sc" :: "q" :: "curPc" :: "curSp" :: "newPc" :: "newSp" :: nil) vs 14 sp
+      * queue b p * susps b sc * any.
 
   Theorem sched_extensional : forall sc, HProp_extensional (sched sc).
     reflexivity.
   Qed.
 
-  Theorem sched_fwd : forall sc, sched sc ===> Ex b, Ex p, sc =*> p * (sc ^+ $4) =?> 2 * queue b p * susps b sc * any.
+  Theorem sched_fwd : forall sc, sched sc ===> Ex b, Ex p, Ex sp, Ex vs, (sc ==*> p, sp) * (sc ^+ $8) =?> 2
+    * locals ("rp" :: "sc" :: "q" :: "curPc" :: "curSp" :: "newPc" :: "newSp" :: nil) vs 14 sp
+    * queue b p * susps b sc * any.
     unfold sched; sepLemma.
   Qed.
 
-  Theorem sched_bwd : forall sc, (Ex b, Ex p, sc =*> p * (sc ^+ $4) =?> 2 * queue b p * susps b sc * any) ===> sched sc.
+  Theorem sched_bwd : forall sc, (Ex b, Ex p, Ex sp, Ex vs, (sc ==*> p, sp) * (sc ^+ $8) =?> 2
+    * locals ("rp" :: "sc" :: "q" :: "curPc" :: "curSp" :: "newPc" :: "newSp" :: nil) vs 14 sp
+    * queue b p * susps b sc * any) ===> sched sc.
     unfold sched; sepLemma.
   Qed.
 End Sched.
@@ -106,7 +120,7 @@ Definition hints : TacPackage.
   prepare (sched_fwd, create_stack) (sched_bwd, susps_empty_bwd, susps_add_bwd).
 Defined.
 
-Definition initS : spec := SPEC reserving 11
+Definition initS : spec := SPEC reserving 12
   PRE[_] mallocHeap 0
   POST[R] sched R * mallocHeap 0.
 
@@ -121,19 +135,50 @@ Definition spawnS : spec := SPEC("sc", "pc", "ss") reserving 18
 Definition exitS : spec := SPEC("sc") reserving 12
   PREonly[V] sched (V "sc") * mallocHeap 0.
 
+Definition yieldS : spec := SPEC("sc") reserving 19
+  PRE[V] sched (V "sc") * mallocHeap 0
+  POST[_] sched (V "sc") * mallocHeap 0.
+
+(* Next, some hijinks to prevent unnecessary unfolding of distinct memory cells for the scheduler's stack. *)
+
+Definition stackSize := 21.
+
+Lemma stackSize_bound : natToW stackSize >= natToW 2.
+  unfold stackSize; auto.
+Qed.
+
+Hint Immediate stackSize_bound.
+
+Lemma stackSize_split : stackSize = length ("rp" :: "sc" :: "q" :: "curPc" :: "curSp" :: "newPc" :: "newSp" :: nil) + 14.
+  reflexivity.
+Qed.
+
+Opaque stackSize.
+
 Definition m := bimport [[ "malloc"!"malloc" @ [mallocS],
     "queue"!"init" @ [Queue.initS], "queue"!"isEmpty" @ [isEmptyS],
     "queue"!"enqueue" @ [enqueueS], "queue"!"dequeue" @ [dequeueS] ]]
   bmodule "scheduler" {{
-    bfunction "init"("q", "r") [initS]
+    (*bfunction "init"("q", "sp", "r") [initS]
       "q" <-- Call "queue"!"init"()
       [PRE[_, R] mallocHeap 0
-       POST[R'] R' =*> R * (R' ^+ $4) =?> 2 * mallocHeap 0];;
+       POST[R'] Ex sp, Ex vs, (R' ==*> R, sp) * (R' ^+ $8) =?> 2
+         * locals ("rp" :: "sc" :: "q" :: "curPc" :: "curSp" :: "newPc" :: "newSp" :: nil) vs 14 sp
+         * mallocHeap 0];;
 
-      "r" <-- Call "malloc"!"malloc"(0, 3)
-      [PRE[V, R] R =?> 3
-       POST[R'] [| R' = R |] * R =*> V "q" * (R ^+ $4) =?> 2 ];;
+      "sp" <-- Call "malloc"!"malloc"(0, stackSize)
+      [PRE[V, R] R =?> stackSize * mallocHeap 0
+        POST[R'] Ex vs, (R' ==*> V "q", R) * (R' ^+ $8) =?> 2 * mallocHeap 0
+         * locals ("rp" :: "sc" :: "q" :: "curPc" :: "curSp" :: "newPc" :: "newSp" :: nil) vs 14 R];;
+
+      Assert [PRE[V] mallocHeap 0
+        POST[R] (R ==*> V "q", V "sp") * (R ^+ $8) =?> 2 * mallocHeap 0];;
+
+      "r" <-- Call "malloc"!"malloc"(0, 4)
+      [PRE[V, R] R =?> 4
+       POST[R'] [| R' = R |] * (R ==*> V "q", V "sp") * (R ^+ $8) =?> 2 ];;
       "r" *<- "q";;
+      "r" + 4 *<- "sp";;
       Return "r"
     end with bfunction "spawnWithStack"("sc", "pc", "sp") [spawnWithStackS]
       "sc" <-* "sc";;
@@ -162,12 +207,13 @@ Definition m := bimport [[ "malloc"!"malloc" @ [mallocS],
       [PRE[_] Emp
        POST[_] Emp];;
       Return 0
-    end with bfunctionNoRet "exit"("sc", "q", "r") [exitS]
-      "q" <-* "sc";;
+    end with*) bfunctionNoRet "exit"("sc", "q", "r") [exitS]
+      Diverge
+      (*"q" <-* "sc";;
       "r" <-- Call "queue"!"isEmpty"("q")
       [Al q,
         PREonly[V, R] [| (q %= empty) \is R |]
-          * queue q (V "q") * V "sc" =*> V "q" * (V "sc" ^+ $4) =?> 2 * susps q (V "sc") * mallocHeap 0];;
+          * queue q (V "q") * (V "sc" ^+ $8) =?> 2 * susps q (V "sc") * mallocHeap 0];;
 
       If ("r" = 1) {
         (* No threads left to run.  Let's loop forever! *)
@@ -175,15 +221,70 @@ Definition m := bimport [[ "malloc"!"malloc" @ [mallocS],
       } else {
         (* Pick a thread to switch to. *)
 
-        "r" <- "sc" + 4;;
+        "r" <- "sc" + 8;;
         Call "queue"!"dequeue"("q", "r")
-        [Al q, Al pc, Al sp,
+        [Al q, Al tsp, Al pc, Al sp,
           PREonly[V] [| (pc, sp) %in q |] * queue (q %- (pc, sp)) (V "q")
             * susps (q %- (pc, sp)) (V "sc") * susp (V "sc") pc sp
-            * (V "sc" ==*> V "q", pc, sp) * mallocHeap 0];;
+            * (V "sc" ==*> V "q", tsp, pc, sp) * mallocHeap 0];;
 
-        Rp <-* "sc" + 4;;
-        Sp <-* "sc" + 8;;
+        Rp <-* "sc" + 8;;
+        Sp <-* "sc" + 12;;
+        IGoto* [("scheduler","exit")] Rp
+      }*)
+    end with bfunction "yield"("sc", "q", "curPc", "curSp", "newPc", "newSp") [yieldS]
+      "q" <-* "sc";;
+      (* Using "curPc" as a temporary before getting to its primary use... *)
+      "curPc" <-- Call "queue"!"isEmpty"("q")
+      [Al q, Al tsp, Al vs,
+        PRE[V, R] [| (q %= empty) \is R |]
+          * queue q (V "q") * (V "sc" ==*> V "q", tsp) * (V "sc" ^+ $8) =?> 2 * susps q (V "sc") * mallocHeap 0
+          * locals ("rp" :: "sc" :: "q" :: "curPc" :: "curSp" :: "newPc" :: "newSp" :: nil) vs 14 tsp * any
+        POST[_] sched (V "sc") * mallocHeap 0];;
+
+      If ("curPc" = 1) {
+        (* No other threads to run.  Simply returning to caller acts like a yield. *)
+        Return 0
+      } else {
+        (* Pick a thread to switch to. *)
+
+        "curPc" <- "sc" + 8;;
+        Call "queue"!"dequeue"("q", "curPc")
+        [Al q, Al tsp, Al vs, Al pc, Al sp,
+          PRE[V] [| (pc, sp) %in q |] * queue (q %- (pc, sp)) (V "q")
+            * susps (q %- (pc, sp)) (V "sc") * susp (V "sc") pc sp
+            * (V "sc" ==*> V "q", tsp, pc, sp) * mallocHeap 0
+            * locals ("rp" :: "sc" :: "q" :: "curPc" :: "curSp" :: "newPc" :: "newSp" :: nil) vs 14 tsp * any
+          POST[_] sched (V "sc") * mallocHeap 0];;
+        "newPc" <-* "sc" + 8;;
+        "newSp" <-* "sc" + 12;;
+
+        Assert [PRE[V] susp (V "sc") (V "newPc") (V "newSp") * sched (V "sc") * mallocHeap 0
+          POST[_] sched (V "sc") * mallocHeap 0];;
+
+        (* Initialize the temporary stack with data we will need, then switch to using it as our stack. *)
+        "curPc" <-* "sc" + 4;;
+        "q" <-* "sc";;
+        "curPc" + 4 *<- "sc";;
+        "curPc" + 8 *<- "q";;
+        "curPc" + 12 *<- $[Sp+0];;
+        "curPc" + 16 *<- Sp;;
+        "curPc" + 20 *<- "newPc";;
+        "curPc" + 24 *<- "newSp";;
+        Sp <- "curPc";;
+
+        Assert [PREonly[V] Ex q, Ex sp, Ex b, (V "sc" ==*> q, sp) * (V "sc" ^+ $8) =?> 2
+          * queue b q * susps b (V "sc") * any * mallocHeap 0
+          * susp (V "sc") (V "newPc") (V "newSp") * susp (V "sc") (V "curPc") (V "curSp")];;
+
+        (* Enqueue current thread; note that variable references below resolve in the temporary stack. *)
+        Call "queue"!"enqueue"("q", "curPc", "curSp")
+        [PREonly[V] Ex sc, sched sc * mallocHeap 0 * susp sc (V "newPc") (V "newSp")];;
+
+        (* Jump to dequeued thread. *)
+        "sc" + 4 *<- Sp;;
+        Rp <-* "newPc";;
+        Sp <-* "newSp";;
         IGoto* [("scheduler","exit")] Rp
       }
     end
@@ -304,7 +405,182 @@ Local Hint Immediate wordBound.
   
 Hint Rewrite <- minus_n_O : sepFormula.
 
+
 Theorem ok : moduleOk m.
+  vcgen.
+
+  (*t.
+  t.
+  t.
+  t.
+  t.
+  t.
+
+  post.
+  evaluate hints.
+  descend.
+  step hints.
+  step hints.
+  step hints.
+  descend; step hints.
+  instantiate (2 := x7).
+  instantiate (3 := upd x1 "q" x8).
+  descend; cancel hints.
+  step hints.
+  step hints.
+  descend; step hints.
+  descend; step hints.
+  descend; step hints.
+  auto.
+  descend; step hints.
+  
+  t.
+  t.
+  t.
+  t.
+  t.
+
+  post.
+  evaluate hints.
+  descend.
+  step hints.
+  2: step hints.
+  eauto.
+  step hints.
+  descend; step hints.
+  instantiate (2 := x2).
+  instantiate (4 := upd (upd x5 "curPc" (Regs x0 Rv)) "curPc" (sel x5 "sc" ^+ $8)).
+  descend; cancel hints.
+  step hints.
+  apply himp_star_frame; [ reflexivity | apply susps_del_fwd; assumption ].
+  step hints.
+  descend; step hints.
+  descend; step hints.
+  descend; step hints.
+  auto.
+  descend; step hints.
+
+  t.
+  t.
+
+  post.
+  evaluate hints.
+  descend.
+  step hints.
+  step hints.
+  step hints.
+  descend; step hints.
+  descend; step hints.
+  auto.
+  descend; step hints.*)
+
+  Focus 17.
+
+  t.
+
+  Focus 17.
+
+  post.
+  evaluate hints.
+  descend.
+  instantiate (2 := upd (upd (upd (upd (upd (upd x5 "sc" (sel x1 "sc")) "q" x7) "curPc"
+    (sel x1 "rp")) "curSp" (Regs x Sp)) "newPc" (sel x1 "newPc")) "newSp" (sel x1 "newSp")); descend.
+  toFront_conc ltac:(fun P => match P with
+                                | susp _ (sel _ "rp") _ => idtac
+                              end).
+  apply susp_intro; descend; eauto.
+  match goal with
+    | [ _ : context[locals ?ns ?v ?a (Regs ?st Sp)] |- interp specs (![?P * _] _) ] =>
+      equate P (locals ns v a (Regs st Sp))
+  end.
+  step hints.
+  big_imp.
+  repeat (apply andL; (apply injL || apply cptrL); intro).
+  apply andL; apply swap; apply andL; apply injL; intro.
+  apply implyR.
+  step hints.
+  auto.
+  
+  step hints.
+
+
+  propxFo.
+  apply andL; apply swap; apply implyR.
+  apply andR; [ apply Imply_I; apply Inj_I; constructor | ].
+
+  repeat ((eapply existsL; intro) || (apply andL; apply injL; intro)).
+  apply 
+
+
+  post.
+  change (locals_call ("rp" :: "sc" :: "q" :: "curPc" :: "curSp" :: "newPc" :: "newSp" :: nil)
+    x1 14 (Regs x Sp) ("rp" :: "b" :: "v1" :: "v2" :: nil) 10 28)
+  with (locals ("rp" :: "sc" :: "q" :: "curPc" :: "curSp" :: "newPc" :: "newSp" :: nil)
+    x1 14 (Regs x Sp)) in H1.
+  generalize dependent H2; evaluate hints; intro.
+  change (locals ("rp" :: "sc" :: "q" :: "curPc" :: "curSp" :: "newPc" :: "newSp" :: nil) x5 14 x6)
+    with (locals_call ("rp" :: "sc" :: "q" :: "curPc" :: "curSp" :: "newPc" :: "newSp" :: nil) x5 14 x6
+      ("rp" :: "b" :: "v1" :: "v2" :: nil) 10 28) in H6.
+  evaluate hints.
+  descend.
+  instantiate (2 := upd (upd (upd x9 "b" x7) "v1" (sel x1 "rp")) "v2" (Regs x Sp)).
+  descend; step hints.
+  step hints.
+  descend; step hints.
+  descend; step hints.
+  
+  instantiate (2 := upd (upd (upd x7 "newPc" x4) "newSp" x5) "curPc" x2).
+  descend; step hints.
+  apply himp_star_frame; [ reflexivity | apply susps_del_fwd; assumption ].
+  step hints.
+  descend; step hints.
+  descend; step hints.
+  descend; step hints.
+  auto.
+  descend; step hints.
+  
+
+
+
+
+
+  t.
+  t.
+  t.
+  t.
+  t.
+
+
+
+
+
+  t.
+  t.
+  t.
+  t.
+  t.
+  t.
+  t.
+  t.
+  t.
+  
+
+  post.
+
+  rewrite stackSize_split in H0.
+  assert (NoDup ("rp" :: "q" :: "curPc" :: "curSp" :: "newPc" :: "newSp" :: nil)) by NoDup.
+  evaluate hints; descend; repeat (step hints; descend); auto.
+
+  t.
+  t.
+  t.
+  t.
+  t.
+
+
+
+
+
   vcgen; try abstract t.
 
 
@@ -365,3 +641,5 @@ Theorem ok : moduleOk m.
       end; clear; descend; step auto_ext.
   step hints; apply any_easy.
 Qed.
+
+Transparent stackSize.
